\begin{sepproof}{Proof of Lemma \ref{gameflow}: Transitive Games Are Flows} \ \\
\label{gameflowproof}
  Let $Sad, Happy, Angry$ be as defined in the Transitive Game. Let $\mathcal{G}'$ be a directed weighted graph based on
  $\mathcal{G}$ with an auxiliary source. Let also $j_1$ be a turn when the Transitive Game has converged. More
  precisely, $\mathcal{G}'$ is defined as follows:
  \begin{equation*}
    \mathcal{V}' = \mathcal{V} \cup \{T\}
  \end{equation*}
  \begin{equation*}
    \mathcal{E}' = \mathcal{E} \cup \{(T, A)\} \cup \{(T, v) : v \in Sad_{j_1}\}
  \end{equation*}
  \begin{equation*}
    \forall (v, w) \in \mathcal{E}, c'_{vw} = DTr_{v \rightarrow w, 0} - DTr_{v \rightarrow w, j_1}
  \end{equation*}
  \begin{equation*}
    \forall v \in Sad_{j_1}, c'_{Tv} = c'_{TA} = \infty
  \end{equation*}
  \subimport{common/figures/}{gameflow.tikz}
  In the figure above, $\mathcal{S}$ is the set of sad players. We observe that $\forall v \in \mathcal{V},$
  \begin{equation}
  \label{gameflowin}
  \begin{gathered}
    \sum\limits_{w \in N^{-}\left(v\right)' \setminus \{T\}}c'_{wv} = \\
    = \sum\limits_{w \in N^{-}\left(v\right)' \setminus \{T\}}\left(DTr_{w \rightarrow v, 0} -
    DTr_{w \rightarrow v, j_1}\right) = \\
    = \sum\limits_{w \in N^{-}\left(v\right)' \setminus \{T\}}DTr_{w \rightarrow v, 0} -
    \sum\limits_{w \in N^{-}\left(v\right)' \setminus \{T\}}DTr_{w \rightarrow v, j-1} =  \\
    = in_{v, 0} - in_{v, j_1}
  \end{gathered}
  \end{equation}
  and
  \begin{equation}
  \label{gameflowout}
  \begin{gathered}
    \sum\limits_{w \in N^{+}\left(v\right)' \setminus \{T\}}c'_{vw} = \\
    = \sum\limits_{w \in N^{+}\left(v\right)' \setminus \{T\}}\left(DTr_{v \rightarrow w, 0} -
    DTr_{v \rightarrow w, j_1}\right) = \\
    = \sum\limits_{w \in N^{+}\left(v\right)' \setminus \{T\}}DTr_{v \rightarrow w, 0} -
    \sum\limits_{w \in N^{+}\left(v\right)' \setminus \{T\}}DTr_{v \rightarrow w, j-1} = \\
    = out_{v, 0} - out_{v, j_1} \enspace.
  \end{gathered}
  \end{equation}
  We can suppose that
  \begin{equation}
  \label{Aincoming}
    \forall j \in \mathbb{N}, in_{A, j} = 0 \enspace,
  \end{equation}
  since if we find a valid flow under this assumption, the flow will still be valid for the original graph. \\
  Next we try to calculate $MaxFlow\left(T, B\right) = X'$ on graph $\mathcal{G}'$. We observe that a flow in which it
  holds that $\forall v, w \in \mathcal{V}, x'_{vw} = c'_{vw}$ can be valid for the following reasons:
  \begin{itemize}
    \item $\forall v,w \in \mathcal{V}, x'_{vw} \leq c'_{vw}$ (Capacity flow requirement (\ref{flow1}) $\forall e \in
    \mathcal{E}$)
    \item Since $\forall v \in Sad_{j_1} \cup \{A\}, c'_{Tv} = \infty$, requirement (\ref{flow1}) holds for any flow
    $x'_{Tv} \geq 0$.
    \item Let $v \in \mathcal{V}' \setminus \left(Sad_{j_1} \cup \{T, A, B\}\right)$. According to the conservative
    strategy and since $v \notin Sad_{j_1},$ it holds that
    \begin{equation*}
      out_{v, 0} - out_{v, j_1} = in_{v, 0} - in_{v, j_1} \enspace.
    \end{equation*}
    Combining this observation with (\ref{gameflowin}) and (\ref{gameflowout}), we have that
    \begin{equation*}
      \sum\limits_{w \in \mathcal{V}'}c'_{vw} = \sum\limits_{w \in \mathcal{V}'}c'_{wv} \enspace.
    \end{equation*}
    (Flow Conservation requirement (\ref{flow2}) $\forall v \in \mathcal{V}' \setminus \left(Sad_{j_1}
    \cup \{T, A, B\}\right)$)
    \item Let $v \in Sad_{j_1}$. Since $v$ is sad, we know that
    \begin{equation*}
      out_{v, 0} - out_{v, j_1} > in_{v, 0} - in_{v, j_1} \enspace.
    \end{equation*}
    Since $c'_{Tv} = \infty$, we can set
    \begin{equation*}
      x'_{Tv} = \left(out_{v, 0} - out_{v, j_1}\right) - \left(in_{v, 0} - in_{v, j_1}\right) \enspace.
    \end{equation*}
    In this way, we have
    \begin{equation*}
      \sum\limits_{w \in \mathcal{V}'}x'_{vw} = out_{v, 0} - out_{v, j_1} \mbox{ and}
    \end{equation*}
    \begin{equation*}
    \begin{gathered}
      \sum\limits_{w \in \mathcal{V}'}x'_{wv} = \sum\limits_{w \in \mathcal{V}' \setminus \{T\}}c'_{wv} + x'_{Tv} =
      in_{v, 0} - in_{v, j_1} + \\ + (out_{v, 0} - out_{v, j_1}) - (in_{v, 0} - in_{v, j_1}) = out_{v, 0} -
      out_{v, j_1} \enspace.
    \end{gathered}
    \end{equation*}
    thus
    \begin{equation*}
      \sum\limits_{w \in \mathcal{V}'}x'_{vw} = \sum\limits_{w \in \mathcal{V}'}x'_{wv} \enspace.
    \end{equation*}
    (Requirement \ref{flow2} $\forall v \in Sad_{j_1}$)
    \item Since $c'_{TA} = \infty$, we can set
    \begin{equation*}
      x'_{TA} = \sum\limits_{v \in \mathcal{V}'}x'_{Av} \enspace,
    \end{equation*}
    thus from (\ref{Aincoming}) we have
    \begin{equation*}
      \sum\limits_{v \in \mathcal{V}'}x'_{vA} = \sum\limits_{v \in \mathcal{V}'}x'_{Av} \enspace.
    \end{equation*}
    (Requirement \ref{flow2} for $A$)
  \end{itemize}
  We saw that for all nodes, the necessary properties for a flow to be valid hold and thus $X'$ is a valid flow for
  $\mathcal{G}$. Moreover, this flow is equal to $maxFlow\left(T, B\right)$ because all incoming flows to $E$ are saturated.
  Also we observe that
  \begin{equation}
  \label{xprimeequalloss}
    \sum\limits_{v \in \mathcal{V}'}x'_{Av} = \sum\limits_{v \in \mathcal{V}'}c'_{Av} = out_{A, 0} - out_{A, j_1} =
    Loss_A \enspace.
  \end{equation}
  We define another graph, $\mathcal{G}''$, based on $\mathcal{G}'$.
  \begin{equation*}
    \mathcal{V}'' = \mathcal{V}'
  \end{equation*}
  \begin{equation*}
    E(\mathcal{G}'') = E(\mathcal{G}') \setminus \{(T, v) : v \in Sad_j\}
  \end{equation*}
  \begin{equation*}
    \forall e \in E(\mathcal{G}''), c''_e = c'_e
  \end{equation*}
  If we execute $MaxFlow(T, B)$ on the graph $\mathcal{G}''$, we will obtain a flow $X''$ in which
  \begin{equation*}
    \sum\limits_{v \in \mathcal{V}''}x''_{Tv} = x''_{TA} = \sum\limits_{v \in \mathcal{V}''}x''_{Av} \enspace.
  \end{equation*}
  The outgoing flow from $A$ in $X''$ will remain the same as in $X'$ for two reasons: Firstly, using the Flow
  Decomposition theorem \cite{amo} and deleting the paths that contain edges $\left(T, v\right): v \neq A$, we
  obtain a flow configuration where the total outgoing flow from $A$ remains invariant,
     \footnote{We thank Kyriakos Axiotis for his insights on the Flow Decomposition theorem.}
  thus
  \begin{equation*}
    \sum\limits_{v \in \mathcal{V}''}x''_{Av} \geq \sum\limits_{v \in \mathcal{V}'}x'_{Av} \enspace.
  \end{equation*}
  Secondly, we have
  \begin{equation*}
    \begin{rcases}
      \sum\limits_{v \in \mathcal{V}''}c''_{Av} = \sum\limits_{v \in \mathcal{V}'}c'_{Av} = \sum\limits_{v \in
      \mathcal{V}'}x'_{Av} \\
      \sum\limits_{v \in \mathcal{V}''}c''_{Av} \geq \sum\limits_{v \in \mathcal{V}''}x''_{Av}
    \end{rcases}
    \Rightarrow \sum\limits_{v \in \mathcal{V}''}x''_{Av} \leq \sum\limits_{v \in \mathcal{V}'}x'_{Av} \enspace.
  \end{equation*}
  Thus we conclude that
  \begin{equation}
  \label{primeequaldoubleprime}
    \sum\limits_{v \in \mathcal{V}''}x''_{Av} = \sum\limits_{v \in \mathcal{V}'}x'_{Av} \enspace.
  \end{equation}
  Let $X = X'' \setminus \{(T, A)\}$. Observe that
  \begin{equation*}
    \sum\limits_{v \in \mathcal{V}''}x''_{Av} = \sum\limits_{v \in \mathcal{V}}x_{Av} \enspace.
  \end{equation*}
  This flow is valid on graph $\mathcal{G}$ because
  \begin{equation*}
    \forall e \in \mathcal{E}, c_e \geq c''_e \enspace.
  \end{equation*}
  Thus there exists a valid flow for each execution of the Transitive Game such that
  \begin{equation*}
    \sum\limits_{v \in \mathcal{V}}x_{Av} = \sum\limits_{v \in \mathcal{V}''}x''_{Av}
    \overset{\left(\ref{primeequaldoubleprime}\right)}{=} \sum\limits_{v \in \mathcal{V}'}x'_{Av}
    \overset{\left(\ref{xprimeequalloss}\right)}{=} Loss_{A, j_1} \enspace,
  \end{equation*}
  which is the flow $X$.
\end{sepproof}
